veric/semax_straight.v
@@ -32,59 +32,6 @@ Transparent intsize_eq.
 Section extensions.
   Context `{!VSTGS OK_ty Σ} {OK_spec : ext_spec OK_ty} {CS: compspecs}.
 
-Definition force_valid_pointers m v1 v2 :=
-match v1, v2 with
-| Vptr b1 ofs1, Vptr b2 ofs2 =>
-    (Mem.valid_pointer m b1 (Ptrofs.unsigned ofs1) &&
-    Mem.valid_pointer m b2 (Ptrofs.unsigned ofs2))%bool
-| _, _ => false
-end.
-
-Lemma mapsto_valid_pointer : forall b o sh t m,
-  sh <> Share.bot ->
-  mem_auth m ∗ mapsto_ sh t (Vptr b o) ⊢
-  ⌜Mem.valid_pointer m b (Ptrofs.unsigned o) = true⌝.
-Proof.
-intros; iIntros "[Hm H]".
-iAssert ⌜exists ch, access_mode t = By_value ch⌝ with "[H]" as %(ch & Hch).
-{ rewrite /mapsto_ /mapsto.
-  destruct (access_mode t) eqn: ?; try done.
-  destruct (type_is_volatile t) eqn: ?; try done.
-  eauto. }
-rewrite /mapsto_ (mapsto_valid_pointer1 _ _ _ _ 0) /offset_val //.
-rewrite Ptrofs.add_zero.
-iMod "H"; iDestruct (valid_pointer_dry with "[$Hm $H]") as %Hvalid.
-by rewrite Z.add_0_r in Hvalid.
-{ pose proof (Ptrofs.unsigned_range o); lia. }
-{ rewrite /sizeof (size_chunk_sizeof _ _ _ Hch).
-  pose proof (size_chunk_pos ch); lia. }
-Qed.
-
-Lemma mapsto_is_pointer : forall sh t v, mapsto_ sh t v ⊢ ⌜exists b, exists o, v = Vptr b o⌝.
-Proof.
-intros. unfold mapsto_, mapsto.
-destruct (access_mode t); try iIntros "[]";
-destruct (type_is_volatile t); try iIntros "[]".
-destruct v; try iIntros "[]".
-iIntros; iPureIntro; eauto.
-Qed.
-
-Lemma is_int_of_bool:
-  forall i s b, is_int i s (Val.of_bool b).
-Proof.
-Transparent Int.repr.
-destruct i,s,b; simpl; auto;
-compute; try split; congruence.
-Opaque Int.repr.
-Qed.
-
-Definition weak_mapsto_ sh e rho :=
-match (eval_expr e rho) with
-| Vptr b o => (mapsto_ sh (typeof e) (Vptr b o)) ∨
-              (mapsto_ sh (typeof e) (Vptr b o))
-| _ => False
-end.
-
 Lemma closed_wrt_modvars_set : forall F id e v ge ve te rho
   (Hclosed : closed_wrt_modvars(Σ:=Σ) (Sset id e) F)
   (Hge : rho = construct_rho (filter_genv ge) ve te),
@@ -266,37 +213,34 @@ forall E (Delta: tycontext) (P: assert) id e t
                             assert_of (subst id (`old) P))).
 Proof.
   intros.
-  apply semax_pre with (▷ tc_expr Delta (Ecast e t) ∧ ▷ P), semax_straight_simple.
-  { intros. rewrite bi.and_elim_r !bi.later_and //. }
-  { apply _. }
-  intros until f; intros TS TC Hcl Hge HGG.
-  assert (typecheck_environ Delta rho) as TYCON_ENV
-    by (destruct TC as [TC' TC'']; eapply typecheck_environ_sub; eauto).
-  iIntros "(Hm & H)".
-  iExists m, (Maps.PTree.set id (eval_expr (Ecast e t) rho) te), _.
-  destruct TS as [TS _]; specialize (TS id).
-  unfold typeof_temp in H99.
-  destruct (temp_types Delta !! id) eqn: Hid; inversion H99; subst t0; clear H99.
-  monPred.unseal.
-  iSplit; [iSplit; first done; iSplit|].
-  + rewrite (bi.and_elim_l (▷ _)) /tc_expr /= typecheck_cast_sound; last apply typecheck_expr_sound; try done.
-    iDestruct "H" as ">%"; iPureIntro.
-    simpl in *. rewrite <- map_ptree_rel.
-    apply guard_environ_put_te'; [subst; auto|].
-    intros ? Hid'; rewrite Hid' in TS; inv TS.
-    by apply tc_val_tc_val'.
-  + iAssert (▷ ⌜Clight.eval_expr ge ve te m (Ecast e t) (eval_expr (Ecast e t) rho)⌝) with "[-]" as ">%"; last by iPureIntro; constructor.
-    iNext; iApply eval_expr_relate; [done..|].
-    iDestruct "H" as "($ & _)"; iFrame.
-  + iIntros "!> !>".
-    iDestruct "H" as "(_ & F & P)"; iFrame.
-    erewrite (closed_wrt_modvars_set F) by eauto; iFrame.
-    iNext; iExists (eval_id id rho).
-    destruct TC as [[TC _] _].
-    destruct (temp_types Delta' !! id) eqn: Hid'; inv TS.
-    destruct (TC _ _ Hid') as (? & ? & ?).
-    super_unfold_lift; erewrite !subst_set by eauto; iFrame.
-    rewrite /eval_id /force_val -map_ptree_rel Map.gss //.
+  rewrite semax_unfold; intros. destruct HGG.
+  iIntros "#? ? #?" (?) "Pre".
+  iApply wp_set.
+  assert (cenv_sub (@cenv_cs CS) psi) by (eapply cenv_sub_trans; eauto).
+  iApply wp_tc_expr; first done.
+  iPoseProof (typecheck_environ_sub' with "[$]") as "#?"; first done.
+  iSplit; first done.
+  iSplit; first by rewrite bi.and_elim_l.
+  iIntros (v ?) "#Hv !>".
+  iStopProof; split => rho; monPred.unseal.
+  rewrite !monPred_at_intuitionistically; monPred.unseal.
+  rewrite {1}/subst /lift1; iIntros "((%TC' & _ & %TC & %) & $ & Pre)".
+  rewrite /typeof_temp in H99; destruct (temp_types Delta !! id) as [t'|] eqn: Ht; inversion H99; subst t'; clear H99.
+  iSplit.
+  - apply TC in Ht as (? & ? & ?).
+    unfold_lift.
+    iExists (eval_id id rho); erewrite !subst_set by done.
+    rewrite !bi.and_elim_r eval_id_same; auto.
+  - rewrite typecheck_cast_sound //.
+    iDestruct "Pre" as "(% & _)".
+    rewrite monPred_at_affinely; iPureIntro.
+    destruct TC' as (? & ? & ?); split3; auto; simpl.
+    intros i t' Ht'; destruct (eq_dec i id).
+    + subst i; destruct TS as (TS & _); specialize (TS id); rewrite Ht Ht' in TS; subst t'.
+      rewrite Map.gss; exists v; subst; split; auto.
+      by apply tc_val_tc_val'.
+    + rewrite Map.gso; auto.
+    + by apply typecheck_expr_sound.
 Qed.
 
 Lemma eval_cast_Vundef:
@@ -310,19 +254,6 @@ Proof.
  try destruct i; try destruct s; try destruct f;
  try destruct i0; try destruct s0; try destruct f0;
  reflexivity.
-Qed.
-
-Lemma eqb_attr_true:
-  forall a a', eqb_attr a a' = true -> a=a'.
-Proof.
-intros.
-destruct a as [v a],a' as [v' a'].
-simpl in H.
-apply andb_true_iff in H.
-destruct H.
-destruct v,v'; inv  H;
-destruct a,a'; inv H0; auto;
-apply Neqb_ok in H1; subst n0; auto.
 Qed.
 
 Lemma semax_load:
@@ -342,53 +273,37 @@ forall E (Delta: tycontext) sh id (P: assert) e1 t2 (v2: val),
 Proof.
   intros until v2.
   intros Hid0 TC1 H_READABLE H99.
-  apply semax_pre with (
-     (▷ tc_lvalue Delta e1 ∧
-      ▷ ⌜tc_val (typeof e1) v2⌝) ∧
-      ▷ P), semax_straight_simple.
-  { intros. rewrite bi.and_elim_r !bi.later_and !assoc //. }
-  { apply _. }
-  intros until f; intros TS TC Hcl Hge HGG.
-  iIntros "(Hm & H)".
-  monPred.unseal.
-  rewrite (bi.and_comm _ (▷⌜_⌝)) -assoc; iDestruct "H" as "(>% & H)".
-  assert (typecheck_environ Delta rho) as TYCON_ENV
-    by (destruct TC as [TC' TC'']; eapply typecheck_environ_sub; eauto).
-  iExists m, (Maps.PTree.set id v2 te), _.
-  destruct TS as [TS _]; specialize (TS id).
-  unfold typeof_temp in Hid0.
-  destruct (temp_types Delta !! id) eqn: Hid; inversion Hid0; subst t; clear Hid0.
-  iSplit; [iSplit; first done; iSplit|].
-  + rewrite (bi.and_elim_l (▷ _)) /tc_lvalue /= typecheck_lvalue_sound; try done.
-    iDestruct "H" as ">%"; iPureIntro.
-    rewrite <- map_ptree_rel.
-    apply guard_environ_put_te'; [subst; auto|].
-    intros ? Hid'; rewrite Hid' in TS; inv TS.
-    by eapply tc_val_tc_val', neutral_cast_subsumption.
-  + iCombine "Hm H" as "H"; rewrite (add_and (_ ∗ _) (▷_)); last by iIntros "H"; iNext; iDestruct "H" as "(Hm & H & _)"; iApply (eval_lvalue_relate with "[$Hm $H]").
-    iDestruct "H" as "((Hm & H) & >%Heval)".
-    destruct Heval as (b & ofs & ? & He1).
-    iAssert (▷ <absorb> mapsto sh (typeof e1) (eval_lvalue e1 rho) v2) with "[H]" as "H".
-    { iNext; iDestruct "H" as "(_ & _ & H)".
-      inversion H99 as [H']. setoid_rewrite monPred_at_absorbingly in H'; iApply H'; monPred.unseal; auto. }
-    rewrite (add_and (▷ _) (▷ _)); last by rewrite mapsto_pure_facts.
-    iDestruct "H" as "(H & >%Hty)".
-    destruct Hty as ((ch & ?) & ?).
-    rewrite He1 mapsto_core_load; try done.
-    iAssert (▷ ⌜load ch m b (Ptrofs.unsigned ofs) = Some v2⌝) with "[-]" as ">%".
-    { iNext; rewrite absorbing; iApply core_load_load'; iFrame. }
-    iPureIntro; constructor; econstructor; eauto.
-    eapply Clight.deref_loc_value; eauto.
-    { by intros ->; eapply tc_val_Vundef. }
-  + iIntros "!> !>".
-    iDestruct "H" as "(_ & F & P)"; iFrame.
-    erewrite (closed_wrt_modvars_set F) by eauto; iFrame.
-    iNext; iExists (eval_id id rho); iSplit.
-    * rewrite /lift1 /eval_id -map_ptree_rel /= Map.gss //.
-    * destruct TC as [[TC _] _].
-      destruct (temp_types Delta' !! id) eqn: Hid'; inv TS.
-      destruct (TC _ _ Hid') as (? & ? & ?).
-      super_unfold_lift; erewrite !subst_set by eauto; iFrame.
+  rewrite semax_unfold; intros; iIntros "#? F #?" (?) "Pre"; destruct HGG.
+  iApply wp_set.
+  assert (cenv_sub (@cenv_cs CS) psi) by (eapply cenv_sub_trans; eauto).
+  rewrite bi.and_comm -assoc bi.later_and; iDestruct "Pre" as "(>%Htc2 & Pre)".
+  iApply wp_expr_mapsto; iApply wp_tc_lvalue; first done.
+  iPoseProof (typecheck_environ_sub' with "[$]") as "#?"; first done.
+  iSplit; first done; iSplit; first by rewrite bi.and_elim_r.
+  iIntros (b o) "#Hbo".
+  iExists sh, v2; iSplit.
+  { iPureIntro; split; first done. intros ->; eapply tc_val_Vundef; eauto. }
+  iSplit.
+  { iNext; iPoseProof (H99 with "[Pre]") as "H".
+    { rewrite bi.and_elim_l; auto. }
+    iStopProof; split => rho; monPred.unseal; rewrite monPred_at_intuitionistically !monPred_at_absorbingly /=; unfold_lift.
+    iIntros "((_ & _ & _ & %Hbo) & _ & H)"; rewrite Hbo //. }
+  iNext; iStopProof; split => rho; monPred.unseal.
+  rewrite !monPred_at_intuitionistically; monPred.unseal.
+  rewrite {1}/subst /lift1; iIntros "((%TC' & _ & %TC & %) & $ & Pre)".
+  rewrite /typeof_temp in Hid0; destruct (temp_types Delta !! id) as [t'|] eqn: Ht; inversion Hid0; subst t'; clear Hid0.
+  iSplit.
+  - apply TC in Ht as (? & ? & ?).
+    unfold_lift.
+    iExists (eval_id id rho); erewrite !subst_set by done.
+    rewrite eval_id_same bi.and_elim_l; auto.
+  - rewrite monPred_at_affinely; iPureIntro.
+    destruct TC' as (? & ? & ?); split3; auto; simpl.
+    intros i t' Ht'; destruct (eq_dec i id).
+    + subst i; destruct TS as (TS & _); specialize (TS id); rewrite Ht Ht' in TS; subst t'.
+      rewrite Map.gss; exists v2; subst; split; auto.
+      eapply tc_val_tc_val', neutral_cast_subsumption; eauto.
+    + rewrite Map.gso; auto.
 Qed.
 
 Lemma mapsto_tc' : forall sh t p v, mapsto sh t p v ⊢ ⌜tc_val' t v⌝.
@@ -427,58 +342,49 @@ forall E (Delta: tycontext) sh id (P: assert) e1 t1 (v2: val),
 Proof.
   intros until v2.
   intros Hid0 HCAST H_READABLE H99.
-  apply semax_pre with (
-     (▷ tc_lvalue Delta e1 ∧
-      ▷ local (`(tc_val t1) (`(eval_cast (typeof e1) t1 v2)))) ∧
-      ▷ P), semax_straight_simple.
-  { intros. rewrite bi.and_elim_r !bi.later_and !assoc //. }
-  { apply _. }
-  intros until f; intros TS TC Hcl Hge HGG.
-  iIntros "(Hm & H)".
-  monPred.unseal.
-  rewrite (bi.and_comm _ (▷⌜_⌝)) -assoc; iDestruct "H" as "(>% & H)".
-  assert (typecheck_environ Delta rho) as TYCON_ENV
-    by (destruct TC as [TC' TC'']; eapply typecheck_environ_sub; eauto).
-  iExists m, (Maps.PTree.set id (eval_cast (typeof e1) t1 v2) te), _.
-  destruct TS as [TS _]; specialize (TS id).
-  unfold typeof_temp in Hid0.
-  destruct (temp_types Delta !! id) eqn: Hid; inversion Hid0; subst t; clear Hid0.
-  iSplit; [iSplit; first done; iSplit|].
-  + iPureIntro.
-    rewrite <- map_ptree_rel.
-    apply guard_environ_put_te'; [subst; auto|].
-    intros ? Hid'; rewrite Hid' in TS; inv TS.
-    by eapply tc_val_tc_val'.
-  + iCombine "Hm H" as "H"; rewrite (add_and (_ ∗ _) (▷_)); last by iIntros "H"; iNext; iDestruct "H" as "(Hm & H & _)"; iApply (eval_lvalue_relate with "[$Hm $H]").
-    iDestruct "H" as "((Hm & H) & >%Heval)".
-    destruct Heval as (b & ofs & ? & He1).
-    iAssert (▷ <absorb> mapsto sh (typeof e1) (eval_lvalue e1 rho) v2) with "[H]" as "H".
-    { iNext; iDestruct "H" as "(_ & _ & H)".
-      inversion H99 as [H']. setoid_rewrite monPred_at_absorbingly in H'; iApply H'; monPred.unseal; auto. }
-    rewrite (add_and (▷ _) (▷ _)); last by rewrite mapsto_pure_facts.
-    iDestruct "H" as "(H & >%Hty)".
-    destruct Hty as ((ch & ?) & ?).
-    super_unfold_lift.
-    assert (v2 <> Vundef) by (intros ->; setoid_rewrite eval_cast_Vundef in H; eapply tc_val_Vundef; eauto).
-    rewrite (add_and (▷ _) (▷ _)); last by rewrite mapsto_tc.
-    iDestruct "H" as "(H & >%)".
-    rewrite He1 mapsto_core_load; try done.
-    iAssert (▷ ⌜load ch m b (Ptrofs.unsigned ofs) = Some v2⌝) with "[-]" as ">%".
-    { iNext; rewrite absorbing; iApply core_load_load'; iFrame. }
-    iPureIntro. constructor; econstructor; [econstructor|]; eauto.
-    * eapply Clight.deref_loc_value; eauto.
-    * unfold eval_cast, force_val1 in *; super_unfold_lift.
-      destruct ((sem_cast (typeof e1) t1) v2) eqn: Hcast; last by apply tc_val_Vundef in H.
-      apply sem_cast_e1; auto.
-  + iIntros "!> !>".
-    iDestruct "H" as "(_ & F & P)"; iFrame.
-    erewrite (closed_wrt_modvars_set F) by eauto; iFrame.
-    iNext; iExists (eval_id id rho); iSplit.
-    * rewrite /lift1 /eval_id -map_ptree_rel /= Map.gss //.
-    * destruct TC as [[TC _] _].
-      destruct (temp_types Delta' !! id) eqn: Hid'; inv TS.
-      destruct (TC _ _ Hid') as (? & ? & ?).
-      super_unfold_lift; erewrite !subst_set by eauto; iFrame.
+  rewrite semax_unfold; intros; iIntros "#? F #?" (?) "Pre"; destruct HGG.
+  iApply wp_set; iApply wp_cast; first done.
+  iApply wp_expr_mono; first by intros; iIntros "H"; iApply "H".
+  iApply wp_expr_mapsto.
+  assert (cenv_sub (@cenv_cs CS) psi) by (eapply cenv_sub_trans; eauto).
+  destruct (eq_dec v2 Vundef).
+  { subst; iAssert (▷ False) with "[Pre]" as ">[]".
+    iNext; rewrite bi.and_elim_r bi.and_elim_l eval_cast_Vundef.
+    iClear "#"; iStopProof; split => rho; monPred.unseal; apply bi.pure_mono, tc_val_Vundef. }
+  iPoseProof (typecheck_environ_sub' with "[$]") as "#?"; first done.
+  iPoseProof (add_and (local (typecheck_environ Delta) ∧ ▷ _) (▷ ⌜tc_val (typeof e1) v2⌝) with "[Pre]") as "((_ & Pre) & >%)";
+    [| iSplit; [done | iApply "Pre"] |].
+  { iIntros "(#? & _ & _ & H) !>"; iPoseProof (H99 with "[H]") as ">H"; auto.
+    iClear "#"; iStopProof; split => rho; monPred.unseal; by apply mapsto_tc. }
+  iApply wp_tc_lvalue; first done.
+  iSplit; first done; iSplit; first by rewrite !bi.and_elim_l.
+  iIntros (b o) "#Hbo".
+  iExists sh, v2; iSplit; first done.
+  iSplit.
+  { iNext; iPoseProof (H99 with "[Pre]") as "H".
+    { rewrite !bi.and_elim_r; auto. }
+    iStopProof; split => rho; monPred.unseal; rewrite monPred_at_intuitionistically !monPred_at_absorbingly /=; unfold_lift.
+    iIntros "((_ & _ & _ & %Hbo) & _ & H)"; rewrite Hbo //. }
+  iStopProof; split => rho; monPred.unseal.
+  rewrite !monPred_at_intuitionistically; monPred.unseal.
+  rewrite {1}/subst /lift1; unfold_lift; iIntros "((%TC' & _ & %TC & %) & $ & Pre)".
+  rewrite bi.and_comm -assoc bi.later_and; iDestruct "Pre" as "(>%Htc & Pre)".
+  iIntros "!>"; iSplit; first done.
+  destruct (sem_cast (typeof e1) t1 v2) as [v|] eqn: Hcast; last by apply tc_val_Vundef in Htc.
+  iExists v; iSplit; first done; iNext.
+  rewrite /typeof_temp in Hid0; destruct (temp_types Delta !! id) as [t'|] eqn: Ht; inversion Hid0; subst t'; clear Hid0.
+  iSplit.
+  - apply TC in Ht as (? & ? & ?).
+    unfold_lift.
+    iExists (eval_id id rho); erewrite !subst_set by done.
+    rewrite eval_id_same bi.and_elim_l; auto.
+  - rewrite monPred_at_affinely; iPureIntro.
+    destruct TC' as (? & ? & ?); split3; auto; simpl.
+    intros i t' Ht'; destruct (eq_dec i id).
+    + subst i; destruct TS as (TS & _); specialize (TS id); rewrite Ht Ht' in TS; subst t'.
+      rewrite Map.gss; exists v; subst; split; auto.
+      by apply tc_val_tc_val'.
+    + rewrite Map.gso; auto.
 Qed.
 
 Lemma writable0_lub_retainer_Rsh:
@@ -519,67 +425,6 @@ Proof.
   apply Nat2Z.inj; auto.
 Qed.
 
-Lemma mapsto_store': forall t t' m ch ch' v v' sh b o m' (Hsh : writable0_share sh)
-  (Hch : access_mode t = By_value ch) (Hch' : access_mode t' = By_value ch')
-  (Hdec : decode_encode_val_ok ch ch') (Ht' : type_is_volatile t' = false)
-  (Halign : (align_chunk ch' | Ptrofs.unsigned o)%Z) (Htc : tc_val' t' (decode_val ch' (encode_val ch v'))),
-  Mem.store ch m b (Ptrofs.unsigned o) v' = Some m' ->
-  mem_auth m ∗ mapsto sh t (Vptr b o) v ⊢ |==> mem_auth m' ∗ ∃ v'', ⌜decode_encode_val v' ch ch' v''⌝ ∧ mapsto sh t' (Vptr b o) v''.
-Proof.
-  intros; rewrite /mapsto Hch Hch' Ht'.
-  iIntros "[Hm H]".
-  destruct (type_is_volatile t); try done.
-  rewrite -> !if_true by auto.
-  setoid_rewrite if_true; last auto.
-  assert (forall v'', decode_encode_val v' ch ch' v'' -> tc_val' t' v'') as Htc'.
-  { intros ? Hv''; eapply decode_encode_val_fun in Hv''; last apply decode_encode_val_general; subst; auto. }
-  iDestruct "H" as "[(% & ?) | (% & % & ?)]"; (iMod (mapsto_store' _ _ _ _ v' with "[$]") as "[$ (% & %Hv'' & H)]"; [done..|]; iIntros "!>";
-    iExists _; iSplit; first done; destruct (eq_dec v'' Vundef); [iRight | specialize (Htc' _ Hv'' n); iLeft]; eauto).
-Qed.
-
-Ltac dec_enc :=
-match goal with
-[ |- decode_val ?CH _ = ?V] => assert (DE := decode_encode_val_general V CH CH);
-                               apply decode_encode_val_similar in DE; auto
-end.
-
-Lemma load_cast:
- forall (t: type) (e2 : expr) (ch : memory_chunk) rho m,
-   tc_val (typeof e2) (eval_expr e2 rho) ->
-   access_mode t = By_value ch ->
-   mem_auth m ∗ denote_tc_assert (isCastResultType (typeof e2) t e2) rho ⊢
-   ⌜Val.load_result ch
-      (force_val (Cop.sem_cast (eval_expr e2 rho) (typeof e2) t m)) =
-    force_val (Cop.sem_cast (eval_expr e2 rho) (typeof e2) t m)⌝.
-Proof.
-intros.
-assert (size_chunk ch = sizeof t) by (symmetry; apply size_chunk_sizeof; auto).
-unfold sizeof in *.
-iIntros "[Hm H]".
-destruct ch;
- destruct t as [ | [ | | | ] [ | ] | [ | ] | [ | ] | | | | | ]; try done;
-simpl in *;
- destruct (eval_expr e2 rho);
- destruct (typeof e2) as [ | [ | | | ] [ | ] | [ | ] | [ | ] | | | | | ] ;
- try done;
-unfold Cop.sem_cast; simpl;
-destruct Archi.ptr64 eqn:Hp;
-try destruct (Float.to_int f);
-try destruct (Float.to_intu f);
-try destruct (Float.to_long f);
-try destruct (Float.to_longu f);
-try destruct (Float32.to_int f);
-try destruct (Float32.to_intu f);
-try destruct (Float32.to_long f);
-try destruct (Float32.to_longu f);
- auto; simpl;
-try solve [try rewrite Int.sign_ext_idem; auto; simpl; lia];
-try rewrite Int.zero_ext_idem; auto; simpl; try lia;
-try solve [simple_if_tac; auto].
-Qed.
-
-Local Arguments typecheck_expr : simpl never.
-
 Lemma semax_store:
  forall E Delta e1 e2 sh P (WS : writable0_share sh),
    semax OK_spec E Delta
@@ -589,67 +434,26 @@ Lemma semax_store:
           (normal_ret_assert (assert_of (`(mapsto sh (typeof e1)) (eval_lvalue e1) (`force_val (`(sem_cast (typeof e2) (typeof e1)) (eval_expr e2)))) ∗ P)).
 Proof.
   intros.
-  apply semax_pre with
-    (∃ v3: val,
-      (▷ tc_lvalue Delta e1 ∧ ▷ tc_expr Delta (Ecast e2 (typeof e1))) ∧
-      ▷ (assert_of (`(mapsto sh (typeof e1)) (eval_lvalue e1) (`v3)) ∗ P)).
-  { intros; iIntros "[? H]".
-    rewrite /mapsto_ !bi.later_and; eauto. }
-  apply extract_exists_pre; intro v3.
-  apply semax_straight_simple; auto.
-  { apply _. }
-  intros until f; intros TS TC Hcl Hge HGG.
-  iIntros "(Hm & H)".
-  assert (typecheck_environ Delta rho) as TYCON_ENV
-    by (destruct TC as [TC' TC'']; eapply typecheck_environ_sub; eauto).
-  monPred.unseal. unfold_lift.
-  rewrite (add_and (_ ∧ (_ ∗ _)) (▷ ⌜_⌝)).
-  2: { iIntros "(_ & _ & ? & _) !>"; iApply (mapsto_pure_facts with "[$]"). }
-  iDestruct "H" as "(H & >%H)".
-  destruct H as ((ch & ?) & ?); destruct (eval_lvalue e1 rho) eqn: He1; try contradiction.
-  iCombine "Hm H" as "H".
-  rewrite (add_and (_ ∗ _) (▷ ⌜_⌝)).
-  2: { iIntros "(? & _ & _ & ? & _) !>".
-       by iApply (mapsto_can_store with "[$]"). }
-  iDestruct "H" as "((Hm & H) & >%Hstore)".
-  destruct Hstore as (m' & Hstore).
-  iExists m', te, rho.
-  iSplit.
-  + iSplit; first by subst.
-    iSplit; first done.
-    iCombine "Hm H" as "H"; rewrite (add_and (_ ∗ _) (▷_)); last by iIntros "H"; iNext; iDestruct "H" as "(Hm & (H & _) & _)"; iApply (eval_lvalue_relate with "[$Hm $H]").
-    iDestruct "H" as "(H & >%He1')".
-    destruct He1' as (? & ? & ? & He1'); rewrite He1' in He1; inv He1.
-    rewrite /tc_expr /typecheck_expr /=; fold typecheck_expr.
-    rewrite denote_tc_assert_andp.
-    rewrite (add_and (_ ∗ _) (▷_)); last by iIntros "H"; iNext; iDestruct "H" as "(Hm & (_ & H & _) & _)"; iApply (eval_expr_relate with "[$Hm $H]").
-    iDestruct "H" as "(H & >%He2)".
-    rewrite (add_and (_ ∗ _) (▷_)); last by iIntros "H"; iNext; iDestruct "H" as "(? & (_ & H) & _)"; iApply (cast_exists with "[$H]").
-    iDestruct "H" as "(H & >%Hcast)".
-    rewrite (add_and (_ ∗ _) (▷_)); last by iIntros "H"; iNext; iDestruct "H" as "(? & (_ & H & _) & _)"; iApply (typecheck_expr_sound with "[$H]").
-    iDestruct "H" as "(H & >%)".
-    rewrite (add_and (_ ∗ _) (▷_)); last by iIntros "H"; iNext; iDestruct "H" as "(Hm & (_ & _ & H) & _)"; iApply (cop2_sem_cast' with "[$Hm $H]").
-    iDestruct "H" as "(H & >%Hcast')".
-    rewrite Hcast in Hcast'.
-    iPureIntro; econstructor; eauto.
-    eapply assign_loc_value; eauto.
-  + iIntros "!>".
-    rewrite typecheck_expr_sound //.
-    rewrite (bi.and_elim_r (▷ tc_lvalue _ _ _)).
-    iDestruct "H" as "(>%Htc & F & >Hmapsto & P)".
-    subst; iPoseProof (mapsto_store with "[$Hm $Hmapsto]") as ">[? ?]"; [try done..|].
-    { by apply tc_val_tc_val'. }
-    rewrite He1; by iFrame.
+  rewrite semax_unfold; intros; iIntros "#? ? #?" (?) "Pre"; destruct HGG.
+  iApply wp_store.
+  assert (cenv_sub (@cenv_cs CS) psi) by (eapply cenv_sub_trans; eauto).
+  iApply wp_tc_expr; first done.
+  iPoseProof (typecheck_environ_sub' with "[$]") as "#?"; first done.
+  iSplit; first done; iSplit; first by rewrite bi.and_elim_l bi.and_elim_r.
+  iIntros (v ?) "#?".
+  iSplit; first by iPureIntro; apply tc_val_tc_val'.
+  iApply wp_tc_lvalue; first done.
+  iSplit; first done; iSplit; first by rewrite !bi.and_elim_l.
+  iIntros (??) "#?".
+  iExists _; iSplit; first done.
+  iDestruct "Pre" as "(_ & He1 & P)"; iSplitL "He1".
+  { iStopProof; split => rho; monPred.unseal; rewrite monPred_at_intuitionistically.
+    unfold_lift; by iIntros "((_ & _ & _ & _ & ->) & ?)". }
+  iNext; iIntros "He1 !>"; simpl; iFrame.
+  iSplit; last done.
+  iStopProof; split => rho; monPred.unseal; rewrite monPred_at_intuitionistically.
+  unfold_lift; by iIntros "((_ & _ & _ & % & ->) & ?)"; subst.
 Qed.
-
-Definition numeric_type (t: type) : bool :=
-match t with
-| Tint IBool _ _ => false
-| Tint _ _ _ => true
-| Tlong _ _ => true
-| Tfloat _ _ => true
-| _ => false
-end.
 
 Lemma semax_store_union_hack:
      forall
@@ -673,77 +477,25 @@ Lemma semax_store_union_hack:
 Proof.
   intros until P. intros NT AM0 AM' OK WS.
   assert (SZ := decode_encode_val_size _ _ OK).
-  apply semax_pre with
-  (∃ v3: val,
-      (▷ tc_lvalue Delta e1 ∧ ▷ tc_expr Delta (Ecast e2 (typeof e1))) ∧
-      ▷ ((assert_of (`(mapsto sh (typeof e1)) (eval_lvalue e1) (`v3))
-                ∧ assert_of (`(mapsto sh t2) (eval_lvalue e1) (`v3))) ∗ P)).
-  { intros; iIntros "[? H]".
-    rewrite /mapsto_ !bi.later_and; eauto. }
-  apply extract_exists_pre; intro v3.
-  apply semax_straight_simple; auto.
-  { apply _. }
-  intros until f; intros TS TC Hcl Hge HGG.
-  iIntros "(Hm & H)".
-  assert (typecheck_environ Delta rho) as TYCON_ENV
-    by (destruct TC as [TC' TC'']; eapply typecheck_environ_sub; eauto).
-  monPred.unseal; unfold_lift.
-  rewrite (add_and (_ ∧ (_ ∗ _)) (▷ ⌜_⌝)).
-  2: { iIntros "(_ & _ & (_ & ?) & _) !>"; iApply (mapsto_pure_facts with "[$]"). }
-  iDestruct "H" as "(H & >%H)".
-  destruct H as (_ & ?); destruct (eval_lvalue e1 rho) eqn: He1; try contradiction.
-  iCombine "Hm H" as "H".
-  rewrite (add_and (_ ∗ _) (▷ ⌜_⌝)).
-  2: { iIntros "(? & _ & _ & (? & _) & _) !>".
-       iApply (mapsto_can_store with "[$]"); eauto. }
-  iDestruct "H" as "((Hm & H) & >%Hstore)".
-  destruct Hstore as (m' & Hstore).
-  iExists m', te, rho.
-  iSplit.
-  + iSplit; first by subst.
-    iSplit; first done.
-    iCombine "Hm H" as "H"; rewrite (add_and (_ ∗ _) (▷_)); last by iIntros "H"; iNext; iDestruct "H" as "(Hm & (H & _) & _)"; iApply (eval_lvalue_relate with "[$Hm $H]").
-    iDestruct "H" as "(H & >%He1')".
-    destruct He1' as (? & ? & ? & He1'); rewrite He1' in He1; inv He1.
-    rewrite /tc_expr /typecheck_expr /=; fold typecheck_expr.
-    rewrite denote_tc_assert_andp.
-    rewrite (add_and (_ ∗ _) (▷_)); last by iIntros "H"; iNext; iDestruct "H" as "(Hm & (_ & H & _) & _)"; iApply (eval_expr_relate with "[$Hm $H]").
-    iDestruct "H" as "(H & >%He2)".
-    rewrite (add_and (_ ∗ _) (▷_)); last by iIntros "H"; iNext; iDestruct "H" as "(? & (_ & H) & _)"; iApply (cast_exists with "[$H]").
-    iDestruct "H" as "(H & >%Hcast)".
-    rewrite (add_and (_ ∗ _) (▷_)); last by iIntros "H"; iNext; iDestruct "H" as "(? & (_ & H & _) & _)"; iApply (typecheck_expr_sound with "[$H]").
-    iDestruct "H" as "(H & >%)".
-    rewrite (add_and (_ ∗ _) (▷_)); last by iIntros "H"; iNext; iDestruct "H" as "(Hm & (_ & _ & H) & _)"; iApply (cop2_sem_cast' with "[$Hm $H]").
-    iDestruct "H" as "(H & >%Hcast')".
-    rewrite Hcast in Hcast'.
-    iPureIntro; econstructor; eauto.
-    eapply assign_loc_value; eauto.
-  + iIntros "!>".
-    rewrite /tc_expr /= typecheck_expr_sound //.
-    rewrite (bi.and_elim_r (▷ tc_lvalue _ _ _)); iDestruct "H" as "(>%Htc & F & >H & P)".
-    iAssert ⌜type_is_volatile t2 = false ∧ (align_chunk ch' | Ptrofs.unsigned i)%Z⌝ with "[H]" as %[??].
-    { iDestruct "H" as "[_ H]"; rewrite /mapsto AM'.
-      destruct (type_is_volatile t2); first done.
-      rewrite -> if_true by auto.
-      iDestruct "H" as "[(% & H) | (% & % & H)]"; rewrite address_mapsto_align; iDestruct "H" as "[_ %]"; done. }
-    iDestruct "H" as "[Hmapsto _]".
-    rewrite /= /force_val1 in Htc; super_unfold_lift.
-    subst; iPoseProof (mapsto_store' with "[$Hm $Hmapsto]") as ">[$ ?]"; eauto.
-    { set (v := force_val _) in *.
-      rewrite andb_true_iff in NT; destruct NT as [NT NT'].
-      destruct ch, ch'; try contradiction OK;
-        destruct (typeof e1) as [ | [ | | | ] [ | ] | [ | ] | [ | ] | | | | | ]; inv NT; inv AM0;
-        destruct t2 as [ | [ | | | ] [ | ] | [ | ] | [ | ] | | | | | ]; inv NT'; inv AM';
-        destruct v; simpl in *; subst; try contradiction;
-        try apply I;
-        try (apply tc_val_Vundef in TCv; contradiction);
-        rewrite /decode_val proj_inj_bytes; intros ?;
-        match goal with
-        | |- context [Int.sign_ext ?n] => apply (sign_ext_range' n); compute; split; congruence
-        | |- context [Int.zero_ext ?n] => apply (zero_ext_range' n); compute; split; congruence
-        | |- _ => idtac
-        end; done. }
-    rewrite He1; by iFrame.
+  rewrite semax_unfold; intros; iIntros "#? ? #?" (?) "Pre"; destruct HGG.
+  iApply wp_store'; [done..|].
+  assert (cenv_sub (@cenv_cs CS) psi) by (eapply cenv_sub_trans; eauto).
+  iApply wp_tc_expr; first done.
+  iPoseProof (typecheck_environ_sub' with "[$]") as "#?"; first done.
+  iSplit; first done; iSplit; first by rewrite bi.and_elim_l bi.and_elim_r.
+  iIntros (v ?) "#?".
+  iSplit; first by iPureIntro; apply tc_val_tc_val'.
+  iApply wp_tc_lvalue; first done.
+  iSplit; first done; iSplit; first by rewrite !bi.and_elim_l.
+  iIntros (??) "#?".
+  iExists _; iSplit; first by iPureIntro; apply writable_writable0.
+  iDestruct "Pre" as "(_ & He1 & P)"; iSplitL "He1".
+  { iStopProof; split => rho; monPred.unseal; rewrite monPred_at_intuitionistically.
+    unfold_lift; by iIntros "((_ & _ & _ & _ & ->) & ?)". }
+  iNext; iIntros "(% & % & He1) !>"; simpl; iFrame.
+  iSplit; last done; iExists v'.
+  iStopProof; split => rho; monPred.unseal; rewrite monPred_at_intuitionistically.
+  unfold_lift; iIntros "((_ & _ & _ & % & ->) & ?)"; subst; auto.
 Qed.
 
 End extensions.
